revised barrier; signal & wait

pulse/lib/pulse/lib/Pulse.Lib.Barrier.fst
@@ -1,28 +1,426 @@
 module Pulse.Lib.Barrier
 open Pulse.Lib.Pervasives
-module CM = FStar.Algebra.CommMonoid
-module M = Pulse.Lib.PCM.MonoidShares
+module PM = Pulse.Lib.PCMMap
+module PF = Pulse.Lib.PCM.Fraction
 module U32 = FStar.UInt32
+module GR = Pulse.Lib.GhostReference
+module OR = Pulse.Lib.OnRange
 #push-options "--using_facts_from '* -FStar.Tactics -FStar.Reflection' --fuel 0 --ifuel 2"
+let small_vprop_map = PM.pointwise nat (PF.pcm_frac #small_vprop)
+let carrier = PM.map nat (PF.fractional small_vprop)
+let small_emp : small_vprop = cm_small_vprop.unit
+noeq
+type barrier_t_core = {
+  r: Box.box U32.t;
+  ctr : GR.ref nat;
+  gref: ghost_pcm_ref small_vprop_map;
+}
 
-let identity_frame_compatible
-      #a (p:FStar.PCM.pcm a)
-      (x:a)
-      (v:a{FStar.PCM.compatible p x v})
-: y:a { FStar.PCM.compatible p y v /\ FStar.PCM.frame_compatible p x v y }
-= x
+noeq type barrier_t = {
+  core: barrier_t_core;
+  i: iref
+}
+let full_perm : perm = 1.0R
+let empty_map_below (n:nat)
+: carrier
+= Map.map_literal 
+  (fun (k:nat) -> 
+    if k < n
+    then None
+    else Some (small_emp, full_perm))
 
-let big_ghost_read_simple
-    (#a:Type)
-    (#p:FStar.PCM.pcm a)
-    (r:ghost_pcm_ref p)
-    (#x:erased a)
-: stt_ghost (erased (v:a{FStar.PCM.compatible p x v /\ p.refine v}))
-    emp_inames
-    (big_ghost_pcm_pts_to r x)
-    (fun v -> big_ghost_pcm_pts_to r x)
-= big_ghost_read #a #p r x (identity_frame_compatible p x)
 
+let up2_is_small (p:small_vprop)
+  : Lemma (is_small (up2 p))
+          [SMTPat (up2 p)]
+  = up2_is_small p
+
+let predicate_at (m:carrier) (i:nat)
+: boxable
+= match Map.sel m i with
+  | None ->
+    pure False
+  | Some f ->
+    up2 (fst f) ** pure (snd f == 0.5R)
+
+let on_range_is_big (p: nat -> boxable) (i j:nat)
+: Lemma (is_big (OR.on_range p i j))
+        [SMTPat (is_big (OR.on_range p i j))]
+= admit()
+
+let map_invariant (v:U32.t) (m:carrier) (n:nat) (p:storable)
+: boxable
+= if v = 0ul
+  then pure (eq2 #storable p (OR.on_range (predicate_at m) 0 n))
+  else OR.on_range (predicate_at m) 0 n
+
+let barrier_inv (b: barrier_t_core) (p:storable)
+: boxable
+= exists* v n m.
+    Box.pts_to b.r #0.5R v **
+    GR.pts_to #nat b.ctr n **
+    big_ghost_pcm_pts_to b.gref m **
+    big_ghost_pcm_pts_to b.gref (empty_map_below n) **
+    map_invariant v m n p
+
+let barrier (b: barrier_t) (p:storable)
+: vprop
+= inv b.i (barrier_inv b.core p)
+
+let send (b: barrier_t) (p:storable)
+: vprop
+= barrier b p **
+  Box.pts_to b.core.r #0.5R 0ul
+
+let singleton (i:nat) (#p:perm) (q:storable)
+: carrier
+= Map.map_literal 
+    (fun (k:nat) ->
+        if k = i
+        then Some (down2 q, p)
+        else None)
+
+let recv (b:barrier_t) (q:storable)
+: vprop
+= exists* p i.
+    barrier b p **
+    big_ghost_pcm_pts_to b.core.gref (singleton i #0.5R q)
+
+let comp (c0:carrier) (c1:carrier { PM.composable_maps (PF.pcm_frac #small_vprop) c0 c1 })
+: carrier 
+= PM.compose_maps (PF.pcm_frac #small_vprop) c0 c1
+
+let initial_map (p:storable)
+: c:carrier { small_vprop_map.refine c }
+= comp (singleton 0 #1.0R p) (empty_map_below 1)
+
+
+```pulse
+ghost
+fn intro_init_map_invariant (p:storable) (q:perm)
+requires emp
+ensures map_invariant 0ul (singleton 0 #q p) 1 p
+{
+  admit()
+}
+```
+
+
+#push-options "--print_implicits"
+```pulse
+fn new_barrier (p:storable)
+requires emp
+returns b:barrier_t
+ensures send b p ** recv b p
+{
+  let r = Box.alloc 0ul;
+  let ctr = GR.alloc #nat 1;
+  let gref = big_ghost_alloc #_ #small_vprop_map (initial_map p);
+  big_ghost_share gref (singleton 0 #1.0R p) (empty_map_below 1);
+  assert pure (singleton 0 #1.0R p `Map.equal` comp (singleton 0 #0.5R p) (singleton 0 #0.5R p));
+  rewrite each (singleton 0 #1.0R p) 
+          as (comp (singleton 0 #0.5R p) (singleton 0 #0.5R p));
+  big_ghost_share gref (singleton 0 #0.5R p) (singleton 0 #0.5R p);
+  Box.share2 r;
+  intro_init_map_invariant p 0.5R;
+  let b = { r; ctr; gref };
+  rewrite each r as b.r, gref as b.gref, ctr as b.ctr;
+  fold (barrier_inv b p);
+  let i = new_invariant (barrier_inv b p);
+  let bb = { core = b; i = i };
+  rewrite each b as bb.core;
+  rewrite each i as bb.i;
+  dup_inv _ _;
+  fold (barrier bb p);
+  fold (send bb p);
+  fold (barrier bb p);
+  with v. rewrite (big_ghost_pcm_pts_to bb.core.gref v) as
+          (big_ghost_pcm_pts_to bb.core.gref (singleton 0 #0.5R p));
+  fold (recv bb p);
+  bb
+}
+```
+
+
+```pulse
+ghost
+fn flip_map_invariant (v:U32.t) (p:storable) (m:carrier) (n:nat)
+requires map_invariant v m n p ** p ** pure (v == 0ul)
+ensures map_invariant 1ul m n p
+{
+  admit()
+}
+```
+
+```pulse
+fn signal (b:barrier_t) (#p:storable)
+requires send b p ** p
+ensures emp
+{
+  unfold send;
+  unfold barrier;
+  with_invariants b.i 
+  returns u:unit
+  ensures inv b.i (barrier_inv b.core p) ** emp
+  {
+    unfold barrier_inv;
+    Box.gather b.core.r;
+    write_atomic_box b.core.r 1ul;
+    Box.share b.core.r;
+    drop_ (Box.pts_to b.core.r #0.5R 1ul);
+    flip_map_invariant _ _ _ _;
+    fold (barrier_inv b.core p);
+  };
+  drop_ (inv b.i _)
+}
+```
+#pop-options
+
+let composable (c0:carrier) (c1:carrier)
+= PM.composable_maps (PF.pcm_frac #small_vprop) c0 c1
+
+let predicate_at_i_is_q_lemma (m:carrier) (i:nat) (n:nat) (q:storable)
+: Lemma
+  (requires
+    composable (singleton i #0.5R q) m /\
+    composable (comp (singleton i #0.5R q) m) (empty_map_below n))
+  (ensures
+    i < n /\
+    (Some? (Map.sel m i) ==> Map.sel m i == (Some (down2 q, 0.5R))))
+= admit()
+
+```pulse
+ghost
+fn elim_on_range_at_i (m:carrier) (i n:nat)
+requires OR.on_range (predicate_at m) 0 n ** pure (i < n)
+ensures OR.on_range (predicate_at m) 0 n ** pure (Some? (Map.sel m i))
+{
+  admit()
+}
+```
+
+```pulse
+ghost
+fn composable_three (gref:ghost_pcm_ref small_vprop_map) (c0 c1 c2:carrier)
+requires big_ghost_pcm_pts_to gref c0 ** big_ghost_pcm_pts_to gref c1 ** big_ghost_pcm_pts_to gref c2
+ensures  big_ghost_pcm_pts_to gref c0 ** big_ghost_pcm_pts_to gref c1 ** big_ghost_pcm_pts_to gref c2
+         ** pure (composable c0 c1 /\ composable (comp c0 c1) c2)
+{
+  big_ghost_gather gref c0 c1;
+  big_ghost_gather gref (comp c0 c1) c2;
+  big_ghost_share gref (comp c0 c1) c2;
+  big_ghost_share gref c0 c1;
+}
+```
+
+module T = FStar.Tactics
+let norm_tac (_:unit) : T.Tac unit =
+    T.mapply (`vprop_equiv_refl)
+
+let elim_predicate_at (m:carrier) (i:nat) 
+: Lemma 
+  (requires Some? (Map.sel m i))
+  (ensures predicate_at m i ==
+           up2 (fst (Some?.v (Map.sel m i))) ** pure (snd (Some?.v (Map.sel m i)) == 0.5R))
+= ()
+
+let apply_equiv (_:unit) : T.Tac unit = 
+  T.dump "A";
+  T.mapply (`vprop_equiv_ext);
+  T.dump "B";
+  T.tadmit()
+  // T.mapply (`elim_predicate_at)
+
+```pulse
+ghost
+fn elim_predicate_at_alt (m:carrier) (i:nat) (_:squash (Some? (Map.sel m i)))
+requires predicate_at m i
+ensures up2 (fst (Some?.v (Map.sel m i))) ** pure (snd (Some?.v (Map.sel m i)) == 0.5R)
+{
+  rewrite_by (predicate_at m i) 
+             (up2 (fst (Some?.v (Map.sel m i))) ** pure (snd (Some?.v (Map.sel m i)) == 0.5R))
+             (apply_equiv) ();
+}
+```
+
+```pulse
+ghost
+fn predicate_at_i_is_q (#gref:ghost_pcm_ref small_vprop_map) (#v:U32.t) (#m:carrier) (#i #n:nat) (#p #q:storable) ()
+requires
+  big_ghost_pcm_pts_to gref (singleton i #0.5R q) **
+  big_ghost_pcm_pts_to gref m **
+  big_ghost_pcm_pts_to gref (empty_map_below n) **
+  map_invariant v m n p **
+  pure (v =!= 0ul)
+ensures
+  big_ghost_pcm_pts_to gref (singleton i #0.5R q) **
+  big_ghost_pcm_pts_to gref m **
+  big_ghost_pcm_pts_to gref (empty_map_below n) **
+  OR.on_range (predicate_at m) 0 i **
+  q **
+  OR.on_range (predicate_at m) (i + 1) n **
+  pure (Map.sel m i == Some (down2 q, 0.5R)) **
+  pure (i < n)
+{
+  rewrite (map_invariant v m n p) as (OR.on_range (predicate_at m) 0 n);
+  composable_three _ _ _ _;
+  predicate_at_i_is_q_lemma m i n q;
+  elim_on_range_at_i m i n;
+  OR.on_range_get i;
+  match Map.sel m i {
+    None -> {
+      rewrite (predicate_at m i) as pure False;
+      unreachable();
+    }
+
+    Some f -> {
+      elim_predicate_at_alt m i ();
+      rewrite (up2 (fst f)) as q;
+      ()
+    }   
+  }
+}
+```
+
+```pulse
+ghost
+fn frame_predicate_at (m0:carrier) (i j:nat) (k:nat) (v:_)
+requires OR.on_range (predicate_at m0) i j ** 
+         pure ((j <= k \/ k < i))
+ensures OR.on_range (predicate_at (Map.upd m0 k v)) i j
+{
+  ghost
+  fn aux (kk:nat { i <= kk /\ kk < j})
+  requires (predicate_at m0 kk)
+  ensures (predicate_at (Map.upd m0 k v) kk)
+  {
+    rewrite (predicate_at m0 kk)
+        as  (predicate_at (Map.upd m0 k v) kk);
+  };
+  OR.on_range_weaken
+    (predicate_at m0)
+    (predicate_at (Map.upd m0 k v))
+    i j
+    aux
+}
+```
+
+```pulse
+ghost
+fn predicate_at_singleton (m:carrier) (i:nat) (q:storable)
+requires q ** pure (Map.sel m i == Some (down2 q, 0.5R))
+ensures predicate_at m i
+{
+  admit()
+}
+```
+
+```pulse
+ghost
+fn clear_i  (#gref:ghost_pcm_ref small_vprop_map) (#m:carrier) (#i #n:nat) (#q:storable) ()
+requires
+  big_ghost_pcm_pts_to gref (singleton i #0.5R q) **
+  big_ghost_pcm_pts_to gref m **
+  pure (Map.sel m i == Some (down2 q, 0.5R)) **
+  OR.on_range (predicate_at m) 0 i **
+  OR.on_range (predicate_at m) (i + 1) n **
+  pure (i < n)
+returns m': erased carrier
+ensures
+  big_ghost_pcm_pts_to gref m' **
+  big_ghost_pcm_pts_to gref (singleton i #0.5R emp) **
+  OR.on_range (predicate_at m') 0 n
+{
+  big_ghost_gather gref _ _;
+  big_ghost_write gref _ _
+    (PM.lift_frame_preserving_upd
+        _ _
+        (PF.mk_frame_preserving_upd (down2 q) (down2 emp))
+        (comp (singleton i #0.5R q) m)
+        i);
+  with m'. assert (big_ghost_pcm_pts_to gref m');
+  assert pure (Map.equal m' (comp (singleton i #0.5R emp) (Map.upd m i (Some (down2 emp, 0.5R)))));
+  rewrite (big_ghost_pcm_pts_to gref m') as
+          (big_ghost_pcm_pts_to gref (comp (singleton i #0.5R emp) (Map.upd m i (Some (down2 emp, 0.5R)))));
+  big_ghost_share gref (singleton i #0.5R emp) (Map.upd m i (Some (down2 emp, 0.5R)));
+  frame_predicate_at m 0 i i (Some (down2 emp, 0.5R));
+  frame_predicate_at m (i + 1) n i (Some (down2 emp, 0.5R));
+  predicate_at_singleton (Map.upd m i (Some (down2 emp, 0.5R))) i emp;
+  OR.on_range_put 0 i n;
+  rewrite (OR.on_range (predicate_at (Map.upd m i (Some (down2 emp, 0.5R)))) 0 n)
+      as  OR.on_range (predicate_at (reveal (hide (Map.upd m i (Some (down2 emp, 0.5R))) ))) 0 n;
+  hide #carrier (Map.upd m i (Some (down2 emp, 0.5R))) 
+}
+```
+
+```pulse
+ghost
+fn fold_barrier_inv (b: barrier_t_core) (p:storable)
+                    (v n m:_)
+requires
+    Box.pts_to b.r #0.5R v **
+    GR.pts_to #nat b.ctr n **
+    big_ghost_pcm_pts_to b.gref m **
+    big_ghost_pcm_pts_to b.gref (empty_map_below n) **
+    map_invariant v m n p
+ensures
+    barrier_inv b p
+{
+  fold barrier_inv
+}
+```
+
+```pulse
+fn rec wait (b:barrier_t) (q:storable)
+requires recv b q
+ensures q
+{
+  unfold recv;
+  with p. assert (barrier b p);
+  with i. assert (big_ghost_pcm_pts_to b.core.gref (singleton i #0.5R q));
+  unfold barrier;
+  let res : bool =
+    with_invariants b.i
+    returns res:bool
+    ensures inv b.i (barrier_inv b.core p) **
+            (cond res q (big_ghost_pcm_pts_to b.core.gref (singleton i #0.5R q)))
+    {
+      unfold barrier_inv;
+      with _v m n. assert (map_invariant _v m n p);
+      let v = read_atomic_box b.core.r;
+      if (v = 0ul)
+      {
+        intro_cond_false
+          q
+          (big_ghost_pcm_pts_to b.core.gref (singleton i #0.5R q));
+        fold (barrier_inv b.core p);
+        false;
+      }
+      else
+      {
+        predicate_at_i_is_q ();
+        let m' = clear_i ();
+        intro_cond_true q (big_ghost_pcm_pts_to b.core.gref (singleton i #0.5R q));
+        fold (map_invariant _v m' n p);
+        fold_barrier_inv _ _ _ _ m';
+        drop_ (big_ghost_pcm_pts_to b.core.gref _);
+        true;
+      }
+    };
+  if res
+  {
+    elim_cond_true _ _ _;
+    drop_ (inv b.i _);
+  }
+  else 
+  {
+    elim_cond_false _ _ _;
+    fold (barrier b p);
+    fold (recv b q);
+    wait b q;
+  }
+}
+```
 
 let small_star = cm_small_vprop.mult
 let small_emp : small_vprop = cm_small_vprop.unit
